pipeline composition where functions can have non-empty arg/retlists
still need to reprove LowerPipeline.flat_to_riscv_correct
to support non-empty arg/retlists, but rest seems done

compiler/src/compiler/Pipeline.v
@@ -14,6 +14,12 @@ Require Export riscv.Utility.Monads.
 Require Import riscv.Utility.runsToNonDet.
 Require Export riscv.Platform.MetricRiscvMachine.
 Require Import coqutil.Z.Lia.
+Require Import coqutil.Tactics.Simp.
+Require Import bedrock2.MetricLogging.
+Require Import compiler.ExprImp.
+Require Import compiler.FlattenExprDef.
+Require Import compiler.FlattenExpr.
+Require Import compiler.FlatImp.
 Require Import compiler.NameGen.
 Require Import compiler.StringNameGen.
 Require Export compiler.util.Common.
@@ -30,199 +36,409 @@ Require Import riscv.Utility.Utility.
 Require Export riscv.Platform.Memory.
 Require Export riscv.Utility.InstructionCoercions.
 Require Import compiler.SeparationLogic.
-Require Import coqutil.Tactics.Simp.
-Require Import compiler.FlattenExprSimulation.
 Require Import compiler.Spilling.
 Require Import compiler.RegAlloc.
 Require Import compiler.FlatToRiscvSimulation.
 Require Import compiler.Simulation.
 Require Import compiler.RiscvEventLoop.
-Require Coq.Init.Byte.
 Require Import bedrock2.MetricLogging.
 Require Import compiler.FlatToRiscvCommon.
 Require Import compiler.FlatToRiscvFunctions.
 Require Import compiler.DivisibleBy4.
 Require Export coqutil.Word.SimplWordExpr.
+Require Export compiler.Registers.
 Require Import compiler.ForeverSafe.
 Require Import FunctionalExtensionality.
 Require Import coqutil.Tactics.autoforward.
 Require Import compiler.FitsStack.
-Require Import compiler.UpperPipeline.
 Require Import compiler.LowerPipeline.
 Import Utility.
 
-Existing Instance riscv.Spec.Machine.DefaultRiscvState.
+Module map.
+  Section WithMap. Local Set Default Proof Using "All".
+    Context {key value} {map : map.map key value} {ok : map.ok map}.
+    Context {key_eqb: key -> key -> bool} {key_eq_dec: EqDecider key_eqb}.
+    Local Hint Mode map.map - - : typeclass_instances.
 
-Open Scope Z_scope.
+    Definition forall_values(P: value -> Prop)(m: map): Prop :=
+      forall k v, map.get m k = Some v -> P v.
+  End WithMap.
+End map.
 
-Section Pipeline1.
-  Context {width: Z}.
-  Context {BW: Bitwidth width}.
-  Context {word: word.word width}.
-  Context {word_ok: word.ok word}.
-  Context {mem: map.map word byte}.
-  Context {Registers: map.map Z word}.
-  Context {string_keyed_map: forall T: Type, map.map string T}. (* abstract T for better reusability *)
-  Context {ext_spec: Semantics.ExtSpec}.
-  Context {M: Type -> Type}.
-  Context {MM: Monad M}.
-  Context {RVM: RiscvProgram M word}.
-  Context {PRParams: PrimitivesParams M MetricRiscvMachine}.
-  Context {word_riscv_ok: RiscvWordProperties.word.riscv_ok word}.
-  Context {string_keyed_map_ok: forall T, map.ok (string_keyed_map T)}.
-  Context {Registers_ok: map.ok Registers}.
-  Context {PR: MetricPrimitives PRParams}.
-  Context {iset: InstructionSet}.
-  Context {BWM: bitwidth_iset width iset}.
-  Context {mem_ok: map.ok mem}.
-  Context {ext_spec_ok: Semantics.ext_spec.ok ext_spec}.
-  Context (compile_ext_call : string_keyed_map Z -> Z -> Z -> FlatImp.stmt Z -> list Instruction).
-  Context (compile_ext_call_correct: forall resvars extcall argvars,
-              compiles_FlatToRiscv_correctly compile_ext_call compile_ext_call
-                                             (FlatImp.SInteract resvars extcall argvars)).
-  Context (compile_ext_call_length_ignores_positions: forall stackoffset posmap1 posmap2 c pos1 pos2,
-              List.length (compile_ext_call posmap1 pos1 stackoffset c) =
-              List.length (compile_ext_call posmap2 pos2 stackoffset c)).
+Section WithWordAndMem.
+  Context {width: Z} {BW: Bitwidth width} {word: Interface.word width} {mem : map.map word byte}.
 
-  Add Ring wring : (word.ring_theory (word := word))
-      (preprocess [autorewrite with rew_word_morphism],
-       morphism (word.ring_morph (word := word)),
-       constants [word_cst]).
+  Record Lang := {
+    Program: Type;
+    Valid: Program -> Prop;
+    Call(p: Program)(funcname: string)(t: trace)(m: mem)(argvals: list word)
+        (post: trace -> mem -> list word -> Prop): Prop;
+  }.
 
-  Local Notation source_env := (string_keyed_map (list string * list string * Syntax.cmd)).
-  Local Notation flat_env := (string_keyed_map (list string * list string * FlatImp.stmt string)).
-  Local Notation renamed_env := (string_keyed_map (list Z * list Z * FlatImp.stmt Z)).
+  Record phase_correct{L1 L2: Lang}{compile: L1.(Program) -> option L2.(Program)}: Prop := {
+    phase_preserves_valid: forall p1 p2,
+        compile p1 = Some p2 ->
+        L1.(Valid) p1 ->
+        L2.(Valid) p2;
+    phase_preserves_post: forall p1 p2,
+        compile p1 = Some p2 ->
+        forall fname t m argvals post,
+        L1.(Call) p1 fname t m argvals post ->
+        L2.(Call) p2 fname t m argvals post;
+  }.
 
-  Definition compile(functions: source_env): option (list Instruction * string_keyed_map Z * Z) :=
-    match upper_compiler functions with
-    | Some functions' => riscvPhase compile_ext_call functions'
+  Arguments phase_correct : clear implicits.
+
+  Definition compose_phases{A B C: Type}(phase1: A -> option B)(phase2: B -> option C)(a: A) :=
+    match phase1 a with
+    | Some b => phase2 b
     | None => None
     end.
 
-  Ltac debool :=
-    repeat match goal with
-           | H: (_ && _)%bool = true |- _ => apply Bool.andb_true_iff in H
-           | H: _ /\ _ |- _ => destruct H as [? H]
-           | H: _ <? _ = true |- _ => eapply Z.ltb_lt in H
-           end.
-
-  Axiom TODO: False.
-
-  Lemma spill_functions_valid_FlatImp_fun: forall funs funs',
-      spill_functions funs = Some funs' ->
-      (forall f argnames retnames body,
-          map.get funs f = Some (argnames, retnames, body) ->
-          NoDup argnames /\ NoDup retnames (* other conditions are checked computationally *)) ->
-      forall f fun_impl,
-      map.get funs' f = Some fun_impl ->
-      FlatToRiscvDef.valid_FlatImp_fun fun_impl.
+  Lemma compose_phases_correct{L1 L2 L3: Lang}
+        {compile12: L1.(Program) -> option L2.(Program)}
+        {compile23: L2.(Program) -> option L3.(Program)}:
+    phase_correct L1 L2 compile12 ->
+    phase_correct L2 L3 compile23 ->
+    phase_correct L1 L3 (compose_phases compile12 compile23).
   Proof.
-    intros. unfold spill_functions in *.
-    eapply map.map_all_values_bw in H. 5: eassumption. all: try typeclasses eauto.
-    unfold spill_fun in H. simp.
-    unfold FlatToRiscvDef.valid_FlatImp_fun, FlatToRiscvDef.valid_FlatImp_var,
-       FlatToRiscvDef.valid_FlatImp_vars,
-       FlatToRiscvDef.valid_FlatImp_var, fp in *.
-    debool.
-    ssplit.
-    - case TODO. (* uses_standard_arg_regs *)
-    - case TODO. (* uses_standard_arg_regs *)
-    - pose proof spill_stmt_valid_vars as P.
-      unfold valid_vars_src, valid_vars_tgt, sp in P.
-(*
-      unfold spill_fbody. cbn. split.
-      { eapply set_vars_to_reg_range_valid_vars.
-      eapply P; clear P. 1: reflexivity.
-      eapply max_var_sound.
-      eapply FlatImp.forallb_vars_stmt_correct.
-      3: eassumption.
-      all: cbv beta; intros; rewrite ?Bool.andb_true_iff, ?Z.ltb_lt; unfold fp; blia.
-    - specialize H0 with (1 := Hp1). eapply H0.
-    - specialize H0 with (1 := Hp1). eapply H0.
-    - case TODO. (* uses_standard_arg_regs *)
-  Qed.
-*)
-  Admitted.
-
-  Lemma regalloc_functions_NoDup: forall funs funs',
-      regalloc_functions funs = Some funs' ->
-      forall f argnames retnames body,
-        map.get funs' f = Some (argnames, retnames, body) -> NoDup argnames /\ NoDup retnames.
-  Proof.
-    unfold regalloc_functions, check_funcs. intros.
-    simp.
-    eapply map.map_all_values_bw in E. 5: eassumption. 2-4: typeclasses eauto.
-    simp.
-    eapply map.get_forallb in E0. 2: eassumption.
-    unfold lookup_and_check_func, check_func, assert in *. simp.
-    autoforward with typeclass_instances in E7. rewrite <- E7.
-    autoforward with typeclass_instances in E6. rewrite <- E6.
-    split; apply List.NoDup_dedup.
+    unfold compose_phases. intros (V12 & C12) (V23 & C23). split; intros; simp; eauto.
   Qed.
 
-  Lemma flatten_functions_NoDup: forall funs funs',
-      (forall f argnames retnames body,
+  Section WithMoreParams.
+    Context {Zlocals: map.map Z word}
+            {string_keyed_map: forall T: Type, map.map string T} (* abstract T for better reusability *)
+            {ext_spec: ExtSpec}
+            {word_ok : word.ok word}
+            {mem_ok: map.ok mem}
+            {string_keyed_map_ok: forall T, map.ok (string_keyed_map T)}
+            {Zlocals_ok: map.ok Zlocals}.
+
+    Context {ext_spec_ok : Semantics.ext_spec.ok ext_spec}.
+
+    (* for riscv phase: *)
+    Context {Registers: map.map Z word}.
+    Context {M: Type -> Type}.
+    Context {MM: Monad M}.
+    Context {RVM: RiscvProgram M word}.
+    Context {PRParams: PrimitivesParams M MetricRiscvMachine}.
+    Context {word_riscv_ok: RiscvWordProperties.word.riscv_ok word}.
+    Context {Registers_ok: map.ok Registers}.
+    Context {PR: MetricPrimitives PRParams}.
+    Context {iset: InstructionSet}.
+    Context {BWM: bitwidth_iset width iset}.
+    Context (compile_ext_call : string_keyed_map Z -> Z -> Z -> FlatImp.stmt Z ->
+                                list Instruction).
+    Context (compile_ext_call_correct: forall resvars extcall argvars,
+                compiles_FlatToRiscv_correctly compile_ext_call compile_ext_call
+                                               (FlatImp.SInteract resvars extcall argvars)).
+    Context (compile_ext_call_length_ignores_positions:
+               forall stackoffset posmap1 posmap2 c pos1 pos2,
+                List.length (compile_ext_call posmap1 pos1 stackoffset c) =
+                List.length (compile_ext_call posmap2 pos2 stackoffset c)).
+
+    Definition locals_based_call_spec{Var Cmd: Type}{locals: map.map Var word}
+               (Exec: string_keyed_map (list Var * list Var * Cmd) ->
+                      Cmd -> trace -> mem -> locals -> MetricLog ->
+                      (trace -> mem -> locals -> MetricLog -> Prop) -> Prop)
+               (e: string_keyed_map (list Var * list Var * Cmd))(f: string)
+               (t: trace)(m: mem)(argvals: list word)
+               (post: trace -> mem -> list word -> Prop): Prop :=
+      exists argnames retnames fbody,
+        map.get e f = Some (argnames, retnames, fbody) /\
+        forall l mc, map.of_list_zip argnames argvals = Some l ->
+                     Exec e fbody t m l mc (fun t' m' l' mc' =>
+                       exists retvals, map.getmany_of_list l' retnames = Some retvals /\
+                                       post t' m' retvals).
+
+    Definition ParamsNoDup{Var: Type}: (list Var * list Var * FlatImp.stmt Var) -> Prop :=
+      fun '(argnames, retnames, body) => NoDup argnames /\ NoDup retnames.
+
+    Definition SrcLang: Lang := {|
+      Program := string_keyed_map (list string * list string * Syntax.cmd);
+      Valid := map.forall_values ExprImp.valid_fun;
+      Call := locals_based_call_spec Semantics.exec;
+    |}.
+    (* |                 *)
+    (* | FlattenExpr     *)
+    (* V                 *)
+    Definition FlatWithStrVars: Lang := {|
+      Program := string_keyed_map (list string * list string * FlatImp.stmt string);
+      Valid := map.forall_values ParamsNoDup;
+      Call := locals_based_call_spec FlatImp.exec;
+    |}.
+    (* |                 *)
+    (* | RegAlloc        *)
+    (* V                 *)
+    Definition FlatWithZVars: Lang := {|
+      Program := string_keyed_map (list Z * list Z * FlatImp.stmt Z);
+      Valid := map.forall_values ParamsNoDup;
+      Call := locals_based_call_spec FlatImp.exec;
+    |}.
+    (* |                 *)
+    (* | Spilling        *)
+    (* V                 *)
+    Definition FlatWithRegs: Lang := {|
+      Program := string_keyed_map (list Z * list Z * FlatImp.stmt Z);
+      Valid := map.forall_values FlatToRiscvDef.valid_FlatImp_fun;
+      Call := locals_based_call_spec FlatImp.exec;
+    |}.
+    (* |                 *)
+    (* | FlatToRiscv     *)
+    (* V                 *)
+    Definition RiscvLang: Lang := {|
+      Program := list Instruction *   (* <- code of all functions concatenated         *)
+                 string_keyed_map Z * (* <- maps function names to instruction offsets *)
+                 Z                    (* <- required stack space in XLEN-bit words     *);
+      Valid _ := True; (* everything is checked by dynamic semantics rather than static ones *)
+      Call := riscv_call;
+    |}.
+
+    Lemma flatten_functions_NoDup: forall funs funs',
+        (forall f argnames retnames body,
           map.get funs f = Some (argnames, retnames, body) -> NoDup argnames /\ NoDup retnames) ->
-      flatten_functions funs = Some funs' ->
-      forall f argnames retnames body,
-        map.get funs' f = Some (argnames, retnames, body) -> NoDup argnames /\ NoDup retnames.
-  Proof.
-    unfold flatten_functions. intros.
-    eapply map.map_all_values_bw in H0. 5: eassumption. 2-4: typeclasses eauto.
-    unfold flatten_function in *. simp.
-    eapply H. eassumption.
-  Qed.
+        flatten_functions funs = Some funs' ->
+        forall f argnames retnames body,
+          map.get funs' f = Some (argnames, retnames, body) -> NoDup argnames /\ NoDup retnames.
+    Proof.
+      unfold flatten_functions. intros.
+      eapply map.map_all_values_bw in H0. 5: eassumption. 2-4: typeclasses eauto.
+      unfold flatten_function in *. simp.
+      eapply H. eassumption.
+    Qed.
 
-  Lemma compiler_correct: forall
-      (stack_start stack_pastend: word)
-      (f_entry_name : string) (fbody: Syntax.cmd.cmd) (f_entry_rel_pos: Z)
-      (p_call p_functions: word)
-      (Rdata Rexec : mem -> Prop)
-      (functions: source_env)
-      (instrs: list Instruction)
-      (pos_map: string_keyed_map Z)
-      (mH: mem)
-      (postH: Semantics.trace -> mem -> Prop)
-      (required_stack_space: Z)
-      (initial: MetricRiscvMachine),
-      ExprImp.valid_funs functions ->
-      compile functions = Some (instrs, pos_map, required_stack_space) ->
-      map.get functions f_entry_name = Some (nil, nil, fbody) ->
-      map.get pos_map f_entry_name = Some f_entry_rel_pos ->
-      required_stack_space <= word.unsigned (word.sub stack_pastend stack_start) / bytes_per_word ->
-      word.unsigned (word.sub stack_pastend stack_start) mod bytes_per_word = 0 ->
-      (forall mc, Semantics.exec functions fbody initial.(getLog) mH map.empty mc
-                                 (fun t' m' l' mc' => postH t' m')) ->
-      machine_ok p_functions f_entry_rel_pos stack_start stack_pastend instrs
-                 p_call p_call mH Rdata Rexec initial ->
-      runsTo initial (fun final => exists mH',
-          postH final.(getLog) mH' /\
-          machine_ok p_functions f_entry_rel_pos stack_start stack_pastend instrs
-                     p_call (word.add p_call (word.of_Z 4)) mH' Rdata Rexec final).
-  Proof.
-    intros. unfold compile in *. simp.
-    pose proof upper_compiler_correct as U. unfold phase_correct, SrcLang, FlatLang in U.
-    edestruct U with (argvals := @nil word) (post := fun t m (_: list word) => postH t m)
-      as (argnames & retnames & fbody' & G' & Sim); clear U.
-    { eassumption. }
-    { do 3 eexists. split. 1: eassumption. unfold map.of_list_zip. simpl. intros. simp.
-      eapply ExprImp.weaken_exec. 1: eauto.
-      cbv beta. intros. exists []. split; [reflexivity|eassumption]. }
-    assert (argnames = []) by case TODO.
-    assert (retnames = []) by case TODO.
-    subst.
-    eapply flat_to_riscv_correct; try typeclasses eauto; try eassumption.
-    { unfold upper_compiler, compose_phases in *. simp.
-      eapply spill_functions_valid_FlatImp_fun. 1: eassumption.
-      eapply regalloc_functions_NoDup. eassumption. }
-    eapply FlatImp.exec.weaken.
-    - eapply Sim. reflexivity.
-    - cbv beta. intros. simp. assumption.
-    Unshelve.
-    all: try exact EmptyMetricLog.
-  Qed.
+    Lemma flattening_correct: phase_correct SrcLang FlatWithStrVars flatten_functions.
+    Proof.
+      unfold SrcLang, FlatWithStrVars.
+      split; cbn. {
+        unfold map.forall_values, ParamsNoDup.
+        intros. destruct v as ((argnames & retnames) & body).
+        eapply flatten_functions_NoDup; try eassumption.
+        unfold valid_fun in *.
+        intros. specialize H0 with (1 := H2). simpl in H0. eapply H0.
+      }
 
-  Definition instrencode(p: list Instruction): list byte :=
-    List.flat_map (fun inst => HList.tuple.to_list (LittleEndian.split 4 (encode inst))) p.
+      unfold locals_based_call_spec. intros. simp.
 
-End Pipeline1.
+      pose proof H as GF.
+      unfold flatten_functions in GF.
+      eapply map.map_all_values_fw in GF. 5: eassumption. 2-4: typeclasses eauto.
+      unfold flatten_function in GF. simp.
+
+      eexists _, _, _. split. 1: eassumption.
+      intros.
+      eapply FlatImp.exec.weaken.
+      - eapply flattenStmt_correct_aux with (mcH := mc).
+        + eassumption.
+        + eauto.
+        + reflexivity.
+        + match goal with
+          | |- ?p = _ => rewrite (surjective_pairing p)
+          end.
+          reflexivity.
+        + intros x k A. assumption.
+        + unfold map.undef_on, map.agree_on. cbn. intros k A.
+          rewrite map.get_empty. destr (map.get l k). 2: reflexivity. exfalso.
+          unfold map.of_list_zip in H0.
+          edestruct (map.putmany_of_list_zip_find_index _ _ _ _ _ _ H0 E) as [G | G]. 2: {
+            rewrite map.get_empty in G. discriminate.
+          }
+          destruct G as (i & G1 & G2).
+          eapply nth_error_In in G1.
+          eapply start_state_spec. 2: exact A.
+          eapply ListSet.In_list_union_l. eapply ListSet.In_list_union_l. assumption.
+        + eapply @freshNameGenState_disjoint_fbody.
+      - simpl. intros. simp. eauto using map.getmany_of_list_extends.
+    Qed.
+
+    Lemma regalloc_functions_NoDup: forall funs funs',
+        regalloc_functions funs = Some funs' ->
+        forall f argnames retnames body,
+          map.get funs' f = Some (argnames, retnames, body) -> NoDup argnames /\ NoDup retnames.
+    Proof.
+      unfold regalloc_functions, check_funcs. intros.
+      simp.
+      eapply map.map_all_values_bw in E. 5: eassumption. 2-4: typeclasses eauto.
+      simp.
+      eapply map.get_forallb in E0. 2: eassumption.
+      unfold lookup_and_check_func, check_func, assert in *. simp.
+      autoforward with typeclass_instances in E7. rewrite <- E7.
+      autoforward with typeclass_instances in E6. rewrite <- E6.
+      split; apply List.NoDup_dedup.
+    Qed.
+
+    Lemma regalloc_correct: phase_correct FlatWithStrVars FlatWithZVars regalloc_functions.
+    Proof.
+      unfold FlatWithStrVars, FlatWithZVars. split; cbn. {
+        unfold map.forall_values, ParamsNoDup. intros.
+        destruct v as ((argnames & retnames) & body).
+        eapply regalloc_functions_NoDup; eassumption.
+      }
+      unfold locals_based_call_spec.
+      intros. simp.
+      pose proof H as GR.
+      unfold regalloc_functions in GR.
+      simp. rename E into GR.
+      eapply map.map_all_values_fw in GR. 5: eassumption. 2-4: typeclasses eauto.
+      simp. clear GRp0.
+      pose proof E0 as C.
+      unfold check_funcs in E0.
+      eapply map.get_forallb in E0. 2: eassumption.
+      unfold lookup_and_check_func, check_func in E0. simp.
+
+      eexists _, _, _. split. 1: reflexivity. intros.
+      unfold map.of_list_zip in *.
+      apply_in_hyps assert_ins_same_length.
+      apply_in_hyps assignments_same_length.
+      apply_in_hyps @map.putmany_of_list_zip_sameLength.
+      assert (List.length argnames = List.length argvals) as P by congruence.
+      eapply map.sameLength_putmany_of_list in P. destruct P as [st2 P].
+      eapply FlatImp.exec.weaken.
+      - eapply checker_correct; eauto.
+        eapply states_compat_precond.
+        edestruct putmany_of_list_zip_states_compat as (lL' & P' & Cp); try eassumption.
+        1: eapply states_compat_empty.
+        rewrite H0 in P'. inversion P'. exact Cp.
+      - simpl. intros. simp. eexists. split. 2: eassumption.
+        destruct u. eauto using states_compat_getmany.
+    Qed.
+
+    Ltac debool :=
+      repeat match goal with
+             | H: (_ && _)%bool = true |- _ => apply Bool.andb_true_iff in H
+             | H: _ /\ _ |- _ => destruct H as [? H]
+             | H: _ <? _ = true |- _ => eapply Z.ltb_lt in H
+             | H: (_ <=? _)%nat = true |- _ => eapply Nat.leb_le in H
+             end.
+
+    Lemma spilling_preserves_valid: forall p1 p2 : string_keyed_map (list Z * list Z * stmt Z),
+        spill_functions p1 = Some p2 ->
+        map.forall_values ParamsNoDup p1 ->
+        map.forall_values FlatToRiscvDef.valid_FlatImp_fun p2.
+    Proof.
+      unfold spill_functions, map.forall_values. intros.
+      eapply map.map_all_values_bw in H. 5: eassumption. all: try typeclasses eauto.
+      unfold spill_fun in H. simp.
+      unfold FlatToRiscvDef.valid_FlatImp_fun, FlatToRiscvDef.valid_FlatImp_var,
+      FlatToRiscvDef.valid_FlatImp_vars,
+      FlatToRiscvDef.valid_FlatImp_var, fp in *.
+      debool.
+      ssplit.
+      - rewrite ?List.firstn_length. change (List.length (Registers.reg_class.all _)) with 8%nat.
+        f_equal. blia.
+      - rewrite ?List.firstn_length. change (List.length (Registers.reg_class.all _)) with 8%nat.
+        f_equal. blia.
+      - cbn. ssplit.
+        + blia.
+        + blia.
+        + eapply set_vars_to_reg_range_valid_vars; unfold a0, a7; try blia.
+          eapply List.forallb_to_Forall. 2: eassumption.
+          unfold is_valid_src_var. intros. debool. assumption.
+        + eapply spill_stmt_valid_vars. 1: reflexivity.
+          unfold valid_vars_src.
+          eapply max_var_sound.
+          eapply FlatImp.forallb_vars_stmt_correct.
+          2: eassumption.
+          unfold is_valid_src_var.
+          intros; rewrite ?Bool.andb_true_iff, ?Z.ltb_lt; unfold fp; blia.
+        + eapply set_reg_range_to_vars_valid_vars; unfold a0, a7; try blia.
+          eapply List.forallb_to_Forall. 2: eassumption.
+          unfold is_valid_src_var. intros. debool. assumption.
+      - cbn. ssplit.
+        + apply set_vars_to_reg_range_uses_standard_arg_regs.
+        + apply spill_stmt_uses_standard_arg_regs.
+        + apply set_reg_range_to_vars_uses_standard_arg_regs.
+    Qed.
+
+    Lemma spilling_correct: phase_correct FlatWithZVars FlatWithRegs spill_functions.
+    Proof.
+      unfold FlatWithZVars, FlatWithRegs. split; cbn. 1: exact spilling_preserves_valid.
+      unfold locals_based_call_spec. intros. simp.
+      pose proof H as GL.
+      unfold spill_functions in GL.
+      eapply map.map_all_values_fw in GL. 5: eassumption. 2-4: typeclasses eauto.
+      destruct GL as (((argnames2 & retnames2) & fbody2) & Sp & G2).
+      exists argnames2, retnames2, fbody2.
+      split. 1: exact G2.
+      eapply spill_fun_correct; eassumption.
+    Qed.
+
+    Lemma riscv_phase_correct: phase_correct FlatWithRegs RiscvLang (riscvPhase compile_ext_call).
+    Proof.
+      unfold FlatWithRegs, RiscvLang.
+      split; cbn. 1: intros; exact I.
+      eapply flat_to_riscv_correct; try eassumption.
+    Qed.
+
+    Definition compile:
+      string_keyed_map (list string * list string * cmd) ->
+      option (list Instruction * string_keyed_map Z * Z) :=
+      (compose_phases flatten_functions
+      (compose_phases regalloc_functions
+      (compose_phases spill_functions
+                      (riscvPhase compile_ext_call)))).
+
+    Lemma composed_compiler_correct: phase_correct SrcLang RiscvLang compile.
+    Proof.
+      unfold compile.
+      exact (compose_phases_correct flattening_correct
+            (compose_phases_correct regalloc_correct
+            (compose_phases_correct spilling_correct
+                                    riscv_phase_correct))).
+    Qed.
+
+    (* restates composed_compiler_correct by unfolding definitions used to compose phases,
+       and turning exists in hyps into toplevel foralls *)
+    Lemma compiler_correct: forall
+        (stack_start stack_pastend: word)
+        (fname: string) (argnames retnames: list string) (fbody: cmd) (f_rel_pos: Z)
+        (p_funcs: word)
+        (Rdata Rexec: mem -> Prop)
+        (functions: string_keyed_map (list string * list string * cmd))
+        (instrs: list Instruction)
+        (pos_map: string_keyed_map Z)
+        (argvals: list word)
+        (mH: mem)
+        (post: trace -> mem -> list word -> Prop)
+        (req_stack_size: Z)
+        (ret_addr: word)
+        (initial: MetricRiscvMachine),
+        ExprImp.valid_funs functions -> (* <-- TODO: why unused? *)
+        compile functions = Some (instrs, pos_map, req_stack_size) ->
+        map.get functions fname = Some (argnames, retnames, fbody) ->
+        map.get pos_map fname = Some f_rel_pos ->
+        req_stack_size <= word.unsigned (word.sub stack_pastend stack_start) / bytes_per_word ->
+        word.unsigned (word.sub stack_pastend stack_start) mod bytes_per_word = 0 ->
+        (forall l mc,
+              map.of_list_zip argnames argvals = Some l ->
+              Semantics.exec functions fbody initial.(getLog) mH l mc
+                (fun t' m' l' mc' => exists retvals: list word,
+                     map.getmany_of_list l' retnames = Some retvals /\ post t' m' retvals)) ->
+        map.get (getRegs initial) RegisterNames.ra = Some ret_addr ->
+        map.getmany_of_list initial.(getRegs)
+                            (List.firstn (Datatypes.length argvals) (reg_class.all reg_class.arg))
+        = Some argvals ->
+        machine_ok p_funcs stack_start stack_pastend instrs
+                   (word.add p_funcs (word.of_Z f_rel_pos)) mH Rdata Rexec initial ->
+        runsTo initial (fun final : MetricRiscvMachine =>
+             exists mH' retvals,
+               map.getmany_of_list (getRegs final)
+                  (List.firstn (List.length retvals) (reg_class.all reg_class.arg))
+               = Some retvals /\
+               post final.(getLog) mH' retvals /\
+               machine_ok p_funcs stack_start stack_pastend instrs ret_addr mH' Rdata Rexec final).
+    Proof.
+      intros.
+      pose proof (phase_preserves_post composed_compiler_correct) as C.
+      match goal with H: _ |- _ => specialize C with (1 := H) end.
+      unfold Call, SrcLang, RiscvLang, locals_based_call_spec, riscv_call in C.
+      edestruct C as (f_rel_pos' & G' & D); clear C. 1: eauto.
+      assert (f_rel_pos' = f_rel_pos) by congruence. subst f_rel_pos'. clear G'.
+      eapply D; clear D; try eassumption.
+    Qed.
+
+    Definition instrencode(p: list Instruction): list byte :=
+      List.flat_map (fun inst => HList.tuple.to_list (LittleEndian.split 4 (encode inst))) p.
+
+  End WithMoreParams.
+End WithWordAndMem.
