compiler/src/compiler/ToplevelLoop.v
@@ -138,7 +138,8 @@ Section Pipeline1.
   (* Holds each time before executing the loop body *)
   Definition ll_good(done: bool)(mach: MetricRiscvMachine): Prop :=
     exists (prog: source_env)
-           (functions_instrs: list Instruction) (positions: string_keyed_map Z) (required_stack_space: Z)
+           (functions_instrs: list Instruction) (positions: string_keyed_map Z)
+           (required_stack_space: Z)
            (init_fun_pos loop_fun_pos: Z) (R: mem -> Prop),
       compile compile_ext_call prog = Some (functions_instrs, positions, required_stack_space) /\
       required_stack_space <= word.unsigned (word.sub (stack_pastend ml) (stack_start ml)) / bytes_per_word /\
@@ -147,13 +148,12 @@ Section Pipeline1.
       map.get positions "loop"%string = Some loop_fun_pos /\
       exists mH,
         isReady spec mach.(getLog) mH /\ goodTrace spec mach.(getLog) /\
-        machine_ok functions_pos loop_fun_pos ml.(stack_start) ml.(stack_pastend) functions_instrs
-                   loop_pos (word.add loop_pos (word.of_Z (if done then 4 else 0))) mH R
-                   (* all instructions which are not part of the loop body (jump to loop body function)
-                      or the compiled functions: *)
-                   (program iset init_sp_pos init_sp_insts *
-                    program iset init_pos (init_insts init_fun_pos) *
-                    program iset backjump_pos backjump_insts)%sep
+        machine_ok functions_pos ml.(stack_start) ml.(stack_pastend) functions_instrs
+                   (word.add loop_pos (word.of_Z (if done then 4 else 0))) mH R
+                   (program iset init_sp_pos (init_sp_insts ++
+                                              init_insts init_fun_pos ++
+                                              loop_insts loop_fun_pos ++
+                                              backjump_insts))
                    mach.
 
   Definition ll_inv: MetricRiscvMachine -> Prop := runsToGood_Invariant ll_good iset.
@@ -162,34 +162,6 @@ Section Pipeline1.
       (preprocess [autorewrite with rew_word_morphism],
        morphism (word.ring_morph (word := word)),
        constants [word_cst]).
-
-  Lemma machine_ok_change_call: forall functions_pos f_entry_rel_pos_1 f_entry_rel_pos_2
-                                       p_stack_start p_stack_pastend instrs
-                                       p_call_1 p_call_2 pc mH Rdata Rexec Rexec1 mach,
-      iff1 Rexec1 (Rexec * ptsto_instr iset p_call_2 (Jal RegisterNames.ra
-                    (f_entry_rel_pos_2 + word.signed (word.sub functions_pos p_call_2))))%sep ->
-      machine_ok functions_pos
-                 f_entry_rel_pos_2
-                 p_stack_start p_stack_pastend instrs
-                 p_call_2
-                 pc mH Rdata
-                 (Rexec * ptsto_instr iset p_call_1 (Jal RegisterNames.ra
-                            (f_entry_rel_pos_1 + word.signed (word.sub functions_pos p_call_1))))%sep
-                 mach ->
-      machine_ok functions_pos
-                 f_entry_rel_pos_1
-                 p_stack_start p_stack_pastend instrs
-                 p_call_1
-                 pc mH Rdata Rexec1
-                 mach.
-  Proof.
-    unfold machine_ok, program.
-    intros. simp; ssplit; eauto.
-    - seprewrite H. wcancel_assumption.
-    - eapply shrink_footpr_subset. 1: eassumption.
-      rewrite H.
-      wwcancel.
-  Qed.
 
   Definition initial_conditions(initial: MetricRiscvMachine): Prop :=
     exists (srcprog: source_env)
@@ -296,26 +268,51 @@ Section Pipeline1.
     end.
     subst.
     intros. simp.
-    (* then, run init_code (using compiler simulation and correctness of init_code) *)
+    (* then, call init function (execute the Jal that jumps there) *)
+    eapply runsToStep. {
+      eapply RunInstruction.run_Jal; cbn.
+      3: solve_word_eq word_ok.
+      3: {
+        eapply rearrange_footpr_subset. 1: eassumption.
+        wwcancel.
+      }
+      { unfold compile, compose_phases, riscvPhase in E. simp.
+        eapply fun_pos_div4 in GetPos. solve_divisibleBy4. }
+      { cbv. auto. }
+      { wcancel_assumption. }
+      { assumption. }
+    }
+    cbn.
+    repeat match goal with
+           | H: valid_machine _ |- _ => clear H
+           end.
+    intros. destruct_RiscvMachine mid. simp.
+    (* then, run body of init function (using compiler simulation and correctness of init) *)
     eapply runsTo_weaken.
     - pose proof compiler_correct compile_ext_call compile_ext_call_correct
                                   compile_ext_call_length_ignores_positions as P.
       unfold runsTo in P.
-      specialize P with (p_functions := word.add loop_pos (word.of_Z 8)) (Rdata := R).
-      unfold ll_good.
+      specialize P with (p_funcs := word.add loop_pos (word.of_Z 8)) (Rdata := R)
+                        (argnames := []) (retnames := []) (argvals := [])
+                        (post := fun t' m' retvals => isReady spec t' m' /\ goodTrace spec t')
+                        (fname := "init"%string).
       eapply P; clear P.
       7: {
+        cbn.
         unfold hl_inv in init_code_correct.
-        simpl.
         move init_code_correct at bottom.
-        subst. intros.
-        refine (init_code_correct _ _ _).
-        replace (datamem_start spec) with (heap_start ml) by congruence.
-        replace (datamem_pastend spec) with (heap_pastend ml) by congruence.
-        exact HMem.
+        intros l' mc OL. cbn in OL. apply Option.eq_of_eq_Some in OL. subst l'.
+        eapply ExprImp.weaken_exec.
+        - refine (init_code_correct _ _ _).
+          replace (datamem_start spec) with (heap_start ml) by congruence.
+          replace (datamem_pastend spec) with (heap_pastend ml) by congruence.
+          exact HMem.
+        - cbv beta. intros * _ _ HP. exists []. split. 1: reflexivity. exact HP.
       }
       all: try eassumption.
-      1: apply stack_length_divisible.
+      { apply stack_length_divisible. }
+      { cbn. apply map.get_put_same. }
+      { reflexivity. }
       unfold machine_ok.
       unfold_RiscvMachine_get_set.
       repeat match goal with
@@ -330,27 +327,8 @@ Section Pipeline1.
         wseplog_pre.
         simpl_addrs.
         subst loop_pos init_pos.
-        match goal with
-        | |- iff1 ?LL ?RR =>
-          match LL with
-          | context[ptsto_instr _ ?A1 (IInstruction (Jal RegisterNames.ra ?J1))] =>
-            match RR with
-            | context[ptsto_instr _ ?A2 (IInstruction (Jal RegisterNames.ra ?J2))] =>
-              unify A1 A2;
-              replace J2 with J1
-            end
-          end
-        end.
-        2: {
-          match goal with
-          | |- context[word.signed ?x] => ring_simplify x
-          end.
-          rewrite signed_of_Z_small.
-          - ring.
-          - clear. cbv. intuition discriminate.
-        }
         wcancel.
-        cancel_seps_at_indices 3%nat 0%nat. {
+        cancel_seps_at_indices 4%nat 0%nat. {
           f_equal.
           solve_word_eq word_ok.
           clear backjump_insts.
@@ -370,25 +348,6 @@ Section Pipeline1.
         wseplog_pre.
         simpl_addrs.
         subst loop_pos init_pos.
-        match goal with
-        | |- iff1 ?LL ?RR =>
-          match LL with
-          | context[ptsto_instr _ ?A1 (IInstruction (Jal RegisterNames.ra ?J1))] =>
-            match RR with
-            | context[ptsto_instr _ ?A2 (IInstruction (Jal RegisterNames.ra ?J2))] =>
-              unify A1 A2;
-              replace J2 with J1
-            end
-          end
-        end.
-        2: {
-          match goal with
-          | |- context[word.signed ?x] => ring_simplify x
-          end.
-          rewrite signed_of_Z_small.
-          - ring.
-          - clear. cbv. intuition discriminate.
-        }
         wcancel.
         cancel_seps_at_indices 0%nat 0%nat. {
           f_equal.
@@ -399,10 +358,13 @@ Section Pipeline1.
         cbn [seps].
         reflexivity.
       }
-      + destruct mlOk. solve_divisibleBy4.
-      + solve_word_eq word_ok.
-      + rapply regs_initialized_put. eassumption.
-      + rewrite map.get_put_same. unfold init_sp. rewrite word.of_Z_unsigned. reflexivity.
+      + unfold compile, compose_phases, riscvPhase in E. simp.
+        eapply fun_pos_div4 in GetPos.
+        destruct mlOk. solve_divisibleBy4.
+      + clear CP. subst loop_pos init_pos init_sp. solve_word_eq word_ok.
+      + do 2 rapply regs_initialized_put. eassumption.
+      + rewrite map.get_put_diff by (cbv; discriminate).
+        rewrite map.get_put_same. unfold init_sp. rewrite word.of_Z_unsigned. reflexivity.
     - cbv beta. unfold ll_good. intros. simp.
       match goal with
       | _: map.get positions "loop"%string = Some ?z |- _ => rename z into f_loop_rel_pos
@@ -418,50 +380,16 @@ Section Pipeline1.
         (* prove that machine_ok of ll_inv (i.e. all instructions, and just before jumping calling
            loop body function) is implied by the state proven by the compiler correctness lemma for
            the init function *)
-        eapply machine_ok_change_call with (p_call_2 := init_pos)
-                                           (f_entry_rel_pos_2 := f_entry_rel_pos).
-        { unfold init_insts, functions_pos, backjump_pos, loop_pos, init_pos.
-          wseplog_pre.
-          cancel.
-          cancel_seps_at_indices 1%nat 1%nat. {
-            f_equal. f_equal. f_equal.
-            match goal with
-            | |- context[word.signed ?x] => ring_simplify x
-            end.
-            rewrite signed_of_Z_small.
-            - ring.
-            - clear. cbv. intuition discriminate.
-          }
-          cbn [seps].
-          reflexivity.
-        }
         lazymatch goal with
-        | H: context[machine_ok] |- ?G => let G' := type of H in replace G with G'; [exact H|clear H]
+        | H: context[machine_ok] |- ?G =>
+          let G' := type of H in replace G with G'; [exact H|clear H]
         end.
         f_equal.
         * unfold functions_pos, backjump_pos. solve_word_eq word_ok.
-        * unfold init_pos. solve_word_eq word_ok.
         * unfold loop_pos, init_pos. solve_word_eq word_ok.
         * eapply iff1ToEq.
+          unfold init_sp_insts, init_insts, loop_insts, backjump_insts.
           wwcancel.
-          cancel_seps_at_indices 1%nat 0%nat. {
-            f_equal. unfold init_sp_insts.
-            solve_word_eq word_ok.
-          }
-          cancel_seps_at_indices 0%nat 0%nat. {
-            f_equal.
-            - unfold loop_pos, init_pos, init_sp_insts. solve_word_eq word_ok.
-            - do 2 f_equal.
-              unfold init_insts, functions_pos, backjump_pos, loop_pos, init_pos.
-              match goal with
-              | |- context[word.signed ?x] => ring_simplify x
-              end.
-              rewrite signed_of_Z_small.
-              + ring.
-              + clear. cbv. intuition discriminate.
-          }
-          cbn [seps].
-          reflexivity.
   Qed.
 
   Lemma ll_inv_is_invariant: forall (st: MetricRiscvMachine),
@@ -515,12 +443,34 @@ Section Pipeline1.
     - solve_word_eq word_ok.
     - unfold ll_good, machine_ok.
       intros. simp. split.
-      + eexists. subst backjump_pos backjump_insts. wcancel_assumption.
+      + eexists. subst loop_pos init_sp_pos init_sp_insts init_pos backjump_pos backjump_insts.
+        wcancel_assumption.
       + eapply shrink_footpr_subset. 1: eassumption.
-        subst backjump_pos backjump_insts.
+        subst loop_pos init_sp_pos init_sp_insts init_pos backjump_pos backjump_insts.
         wwcancel.
-    - (* use compiler correctness for loop body *)
-      intros.
+    - intros. destruct_RiscvMachine initial. unfold ll_good, machine_ok in H. cbn in *. simp.
+      (* call loop function (execute the Jal that jumps there) *)
+      eapply runsToStep. {
+        eapply RunInstruction.run_Jal; cbn.
+        3: reflexivity.
+        3: {
+          eapply rearrange_footpr_subset. 1: eassumption.
+          unfold init_sp_pos, init_sp_insts, loop_pos, init_pos.
+          wwcancel.
+        }
+        { match goal with
+          | H: map.get positions "loop"%string = Some _ |- _ => rename H into GetPos
+          end.
+          unfold compile, compose_phases, riscvPhase in *. simp.
+          eapply fun_pos_div4 in GetPos. solve_divisibleBy4. }
+        { cbv. auto. }
+        { subst loop_pos init_pos init_sp_pos init_sp_insts.
+          wcancel_assumption. }
+        { assumption. }
+      }
+      cbn.
+      intros. destruct_RiscvMachine mid. simp.
+      (* use compiler correctness for loop body *)
       unfold ll_good in *. simp.
       match goal with
       | H: ProgramSatisfiesSpec _ _ _ _ |- _ => pose proof H as sat; destruct H
@@ -537,14 +487,78 @@ Section Pipeline1.
       + pose proof compiler_correct compile_ext_call compile_ext_call_correct
                                     compile_ext_call_length_ignores_positions as P.
         unfold runsTo in P.
+        specialize P with (argnames := []) (retnames := []) (argvals := [])
+                          (fname := "loop"%string)
+                          (post := fun t' m' retvals => isReady spec t' m' /\ goodTrace spec t').
         eapply P; clear P. 7: {
-          intros.
-          eapply loop_body_correct; eauto.
+        cbn.
+        move loop_body_correct at bottom.
+        intros l' mc OL. cbn in OL. apply Option.eq_of_eq_Some in OL. subst l'.
+        eapply ExprImp.weaken_exec.
+        - eapply loop_body_correct; eauto.
+        - cbv beta. intros * _ _ HP. exists []. split. 1: reflexivity. exact HP.
         }
         all: try eassumption.
-        1: apply stack_length_divisible.
+        { apply stack_length_divisible. }
+        { cbn. apply map.get_put_same. }
+        { reflexivity. }
+        unfold machine_ok.
+        unfold_RiscvMachine_get_set.
+        repeat match goal with
+               | x := _ |- _ => subst x
+               end.
+        repeat match goal with
+               | |- exists _, _  => eexists
+               | |- _ /\ _ => split
+               | |- _ => progress cbv beta iota
+               | |- _ => eassumption
+               | |- _ => reflexivity
+               end.
+        * match goal with
+          | H: map.get positions "loop"%string = Some _ |- _ => rename H into GetPos
+          end.
+          unfold compile, compose_phases, riscvPhase in *. simp.
+          eapply fun_pos_div4 in GetPos.
+          remember (word.add
+               (word.add
+                  (word.add (code_start ml)
+                     (word.of_Z
+                        (4 *
+                         Z.of_nat
+                           (Datatypes.length
+                              (FlatToRiscvDef.compile_lit iset RegisterNames.sp
+                                 (word.unsigned (stack_pastend ml)))))))
+                  (word.of_Z 4)) (word.of_Z 0)) as X.
+          solve_divisibleBy4.
+        * solve_word_eq word_ok.
+        * eapply regs_initialized_put. eassumption.
+        * rewrite map.get_put_diff by (cbv; discriminate). assumption.
+        * match goal with
+          | H: valid_machine {| getMetrics := ?M |} |- valid_machine {| getMetrics := ?M |} =>
+            eqexact.eqexact H; f_equal; f_equal
+          end.
+          { f_equal. solve_word_eq word_ok. }
+          { solve_word_eq word_ok. }
+          { solve_word_eq word_ok. }
       + cbv beta.
-        intros. simp. eauto 17.
+        intros.
+        destruct_RiscvMachine final.
+        repeat match goal with
+               | x := _ |- _ => subst x
+               end.
+        unfold machine_ok in *. simpl_MetricRiscvMachine_get_set. simp.
+        simpl_MetricRiscvMachine_get_set.
+        repeat match goal with
+               | |- exists _, _  => eexists
+               | |- _ /\ _ => split
+               | |- _ => progress cbv beta iota
+               | |- _ => eassumption
+               | |- _ => reflexivity
+               end.
+        move Hp10 at bottom.
+        cbn in Hp10.
+        rewrite Hp10.
+        solve_word_eq word_ok.
   Qed.
 
   Lemma ll_inv_implies_prefix_of_good: forall st,
